Strata/DL/Imperative/Imperative.lean
@@ -12,7 +12,6 @@ public import Strata.DL.Imperative.MetaData
 public import Strata.DL.Imperative.CmdEval
 public import Strata.DL.Imperative.CmdType
 public import Strata.DL.Imperative.CmdSemantics
-public import Strata.DL.Imperative.StmtSemantics
 public import Strata.DL.Imperative.StmtSemanticsSmallStep
 
 public import Strata.DL.Imperative.NondetStmt
