Strata/Transform/StructuredToUnstructured.lean
@@ -6,6 +6,7 @@
 
 import Strata.DL.Imperative.PureExpr
 import Strata.DL.Imperative.BasicBlock
+import Strata.DL.Imperative.CFGSemantics
 import Strata.DL.Imperative.Cmd
 import Strata.DL.Imperative.Stmt
 import Strata.DL.Lambda.LExpr
